Refactored poly_result.lean
Induction step generalized over any proposition function F_2[X] -> Prop.

src/IMO2017/A6/A6_char_eq_2/poly_result.lean
@@ -1,8 +1,12 @@
 import
   IMO2017.A6.A6_char_eq_2.basic
-  data.zmod.basic
-  data.polynomial.eval
-  data.polynomial.div
+  IMO2017.A6.A6_char_eq_2.extra.my_F2X_induction
+
+namespace IMO2017A6
+
+universe u
+variable {F : Type u}
+variable [field F]
 
 /-
   The big polynomial result: for any a, b ∈ F, if f(a) = f(b), then
@@ -26,15 +30,13 @@ import
   Together with f(a) = f(b), we get f(Q(a) a) + f(Q(a) + a) = f(Q(b) b) + f(Q(b) + b).
   But Q + X has degree ≤ max(1, deg(Q)) < n.
   Thus, f(Q(a) + a) = f(Q(b) + b), which implies f(Q(a) a) = f(Q(b) b).
+
+
+
+  Implementation details:
+  We will need to rewrite our own induction step for this problem.
+  See file "extra/my_F2X_induction.lean".
 -/
-
-
-
-namespace IMO2017A6
-
-universe u
-variable {F : Type u}
-variable [field F]
 
 
 
@@ -54,7 +56,7 @@ namespace poly_result
 
 open polynomial
 
-def phi2F := zmod.cast_hom (dvd_refl 2)
+def phi2F := zmod.cast_hom (dvd_refl 2) F
 
 
 
@@ -65,81 +67,22 @@ include feq1 feq2
 
 
 
-lemma fn_induction_intro {a b : F} (h : f a = f b) :
-  ∀ P : polynomial (zmod 2),
-    f (eval₂ (phi2F F) a P) = f (eval₂ (phi2F F) b P) →
-      f (eval₂ (phi2F F) a (X + P)) = f (eval₂ (phi2F F) b (X + P)) →
-        f (eval₂ (phi2F F) a (X * P)) = f (eval₂ (phi2F F) b (X * P)) :=
-begin
-  intros P h0 h1,
-  rw [eval₂_add, eval₂_X, eval₂_add, eval₂_X] at h1,
-  rw [eval₂_mul, eval₂_X, eval₂_mul, eval₂_X],
-  let Pa := eval₂ (phi2F F) a P,
-  let Pb := eval₂ (phi2F F) b P,
-  calc f (a * Pa) = f (a * Pa) + f (a + Pa) - f (a + Pa) : by rw add_sub_cancel
-  ... = f (b * Pb) + f (b + Pb) - f (a + Pa) : by rw base_lemma.fn_lem2_7 feq1 feq2 h h0
-  ... = f (b * Pb) : by rw [h1, add_sub_cancel],
-end
-
 theorem fn_thm {a b : F} (h : f a = f b) :
-  ∀ P : polynomial (zmod 2), f (eval₂ (phi2F F) a P) = f (eval₂ (phi2F F) b P) :=
+  ∀ P : polynomial (zmod 2), f (eval₂ phi2F a P) = f (eval₂ phi2F b P) :=
 begin
-
-  ---- Start with describing all the elements of zmod 2
-  have zmod2_elts : ∀ c : zmod 2, c = 0 ∨ c = 1 :=
-  begin
-    intros c,
-    cases c with x x_prop,
-    rcases x with _ | x | x,
-    left; refl,
-    right; refl,
-    rw [nat.succ_lt_succ_iff, nat.add_def, add_zero, nat.succ_lt_succ_iff] at x_prop,
-    exfalso; exact nat.not_lt_zero x x_prop,
-  end,
-
-  ---- Some stupid result
-  have zmod2_coe : ∀ c : zmod 2, (phi2F F) c = ↑c :=
-  begin
-    intros c; cases c,
-    unfold phi2F; rw zmod.cast_hom_apply,
-  end,
-
-  ---- Another stupid result
-  have fn_aux : ∀ (x : F) (c : zmod 2), f (x + c) = f x + c :=
-  begin
-    intros x c,
-    cases zmod2_elts c with h h,
-    rw [h, zmod.cast_zero, add_zero, add_zero],
-    rw [h, zmod.cast_one', feq2],
-  end,
-
-  ---- Start of the main result
-  intros P,
-  induction h0 : P.nat_degree using nat.strong_induction_on with n n_ih generalizing P,
-  cases le_or_lt n 1 with h1 h1,
-
-  -- Case n ≤ 1
-  { rw ← h0 at h1,
-    rw eq_X_add_C_of_nat_degree_le_one h1,
-    simp only [polynomial.eval₂_C, polynomial.eval₂_X, polynomial.eval₂_add, polynomial.eval₂_mul],
-    rw [zmod2_coe, zmod2_coe, fn_aux, fn_aux, add_left_inj],
-    cases zmod2_elts (P.coeff 1) with Px Px; rw Px; simp,
-    exact h, },
-
-  -- Case 1 < n
-  { rw [← mod_by_monic_add_div P monic_X, mod_by_monic_X, add_comm, eval₂_add,
-        eval₂_add, eval₂_C, eval₂_C, zmod2_coe, fn_aux, fn_aux, add_left_inj],
-    suffices : (P /ₘ X).nat_degree < n,
-    { apply fn_induction_intro feq1 feq2 h,
-      { apply n_ih (P /ₘ X).nat_degree this; refl, },
-      { apply n_ih (X + P /ₘ X).nat_degree,
-        swap,
-        refl,
-        apply lt_of_le_of_lt (nat_degree_add_le X _),
-        simp only [nat_degree_X, max_lt_iff],
-        split; assumption, }, },
-    rw [nat_degree_div_by_monic P monic_X, nat_degree_X, h0],
-    exact nat.sub_lt (lt_trans zero_lt_one h1) zero_lt_one, },
+  apply extra.my_F2X_induction.induction1,
+  { rw [eval₂_zero, eval₂_zero] },
+  { rwa [eval₂_X, eval₂_X] },
+  { intros P h,
+    rw [eval₂_add, eval₂_one, feq2, h, eval₂_add, eval₂_one, feq2] },
+  { intros P h0 h1,
+    rw [eval₂_add, eval₂_X, eval₂_add, eval₂_X] at h1,
+    rw [eval₂_mul, eval₂_X, eval₂_mul, eval₂_X],
+    let Pa : F := eval₂ phi2F a P,
+    let Pb : F := eval₂ phi2F b P,
+    calc f (Pa * a) = f (Pa * a) + f (Pa + a) - f (Pa + a) : by rw add_sub_cancel
+    ... = f (Pb * b) + f (Pb + b) - f (Pa + a) : by rw base_lemma.fn_lem2_7 feq1 feq2 h0 h
+    ... = f (Pb * b) : by rw [h1, add_sub_cancel] },
 end
 
 end poly_result
